+++
title = "Laws of Logarithms"
menutitle = "4.3 Laws of Logarithms"
description = "4.3 Notes"
weight = 4
+++

## _Notes:_

### Terms

***The Product Rule:***

***log<sub>a</sub>(x * y) = log<sub>a</sub>(x) + log<sub>a</sub>(y)***

- It's just a rewritten form of: <br/> ***a<sup>r</sup> * a<sup>s</sup> = a<sup>r + s</sup>***

***The Quotient Rule:***

***log<sub>a</sub>(x / y) = log<sub>a</sub>(x) - log<sub>a</sub>(y)***

- It's just a rewritten form of: <br/> ***a<sup>r</sup> / a<sup>s</sup> = a<sup>r - s</sup>***

***The Power Rule:***

***log<sub>a</sub>(x<sup>c</sup>) = C * log<sub>a</sub>(x)***

- It's just a rewritten form of: <br/> ***(a<sup>r)<sup>s</sup></sup> = a<sup>r * s</sup>***

### Theorems/Formulas

***The Change of Base Formula:*** <br/>
**log<sub>a</sub>b** = **ln(b) / ln(a)** = **log(b) / log(a)**

- Proof:
  - ***log<sub>3</sub>(157) = ln(157) / ln(3) ≈ 4.6***

AND

- More Proof:
  - ***log<sub>4</sub>16 = ln(16) / ln(4) ≈ 2***

***Logs of reciprocals are opposite:*** <br/>
**For any value of x, log<sub>a</sub>x = -log<sub>a</sub>(1 / x)**

- Proof of Inverse: <br />
  => ***log<sub>a</sub>(1 / x) = log<sub>a</sub>1 - log<sub>a</sub>(x)***

  => ***log<sub>a</sub>(1 / x) = 0 - log<sub>a</sub>(x)***

  => ***-log<sub>a</sub>(x)***

**log<sub>a</sub>b = 1 / log<sub>b</sub>a**

- More Proof: <br />
  => ***log<sub>25</sub>5 = 0.5***
  
  => ***log<sub>5</sub>25 = 2***
